

No: _____

Date: _____

C6

T1. 证明: (1) 由 $\delta_p(a) = 3$ 可知 $a \bmod p \neq 1$, 故 $p \nmid a-1$,
 $(a-1, p) = 1$, 由 $(a-1) \sum_{k=0}^{p-2} a^k = a^p - 1 \equiv a-1 \pmod p$, 故有
 $\sum_{k=0}^{p-2} a^k \equiv 1 \pmod p$.

(2) 由 $\delta_p(a) = 3$ 得 $a^2 \not\equiv 1 \pmod p$, $a \not\equiv \pm 1 \pmod p$, 由 (1) 中方法可
 证 $1+a+a^2 \equiv 0 \pmod p$, 所以 $1+a \not\equiv 1 \pmod p$, $(1+a)^2 = 1+2a+a^2$
 $\equiv a \not\equiv 1 \pmod p$, $(1+a)^3 = a^3+3a^2+3a+1 \equiv 1+3(a^2+a+1)-2$
 $\equiv -1 \pmod p$, 故 $\delta_p(1+a) = 6$.

T3. 证明: (1) 由已知得 $(ab, n) = 1$,

由 $(ab)^{[\delta_n(a), \delta_n(b)]} = (a^{\delta_n(a)})^{\frac{[\delta_n(a), \delta_n(b)]}{\delta_n(a)}} (b^{\delta_n(b)})^{\frac{[\delta_n(a), \delta_n(b)]}{\delta_n(b)}} \equiv 1 \pmod n$
 得 $\delta_n(ab) \mid [\delta_n(a), \delta_n(b)]$;

又 $(ab)^{\delta_n(ab)\delta_n(b)} \equiv (a^{\delta_n(ab)\delta_n(b)}) \equiv 1 \pmod n$, 故 $\delta_n(a) \mid \delta_n(ab)\delta_n(b)$

从而有 $\frac{\delta_n(a)}{(\delta_n(a), \delta_n(b))} \mid \delta_n(ab)$, 同理有 $\frac{\delta_n(b)}{(\delta_n(a), \delta_n(b))} \mid \delta_n(ab)$.

①充分性 (\Leftarrow): $(\delta_n(a), \delta_n(b)) = 1$, 则 $\delta_n(a) \mid \delta_n(ab)$, $\delta_n(b) \mid \delta_n(ab)$,
 得 $\delta_n(a)\delta_n(b) \mid \delta_n(ab)$. 又 $(ab)^{\delta_n(a)\delta_n(b)} \equiv 1 \pmod n$, $\delta_n(ab) \mid \delta_n(a)\delta_n(b)$
 所以 $\delta_n(ab) = \delta_n(a)\delta_n(b)$

②必要性 (\Rightarrow): 若 $\delta_n(ab) = \delta_n(a)\delta_n(b)$, 则 $\delta_n(a)\delta_n(b) \mid [\delta_n(a), \delta_n(b)]$
 即 $(\delta_n(a), \delta_n(b))[\delta_n(a), \delta_n(b)] \mid [\delta_n(a), \delta_n(b)]$, 可知必有
 $(\delta_n(a), \delta_n(b)) = 1$.

证毕.

T4. (1) 证明: 对 $\forall k, 1 \leq k \leq \frac{p-1}{2}$, $(g^{2k})^{\frac{p-1}{2}} = (g^{p-1})^k \equiv 1 \pmod{p}$

所以 g^2, g^4, \dots, g^{p-1} 为模 p 的二次剩余, 故剩余 $\frac{p-1}{2}$ 个元素 g, g^3, \dots, g^{p-2} 为模 p 的二次非剩余.

T6. (1) 证明: $2 \mid p-1$, 故 $(-g)^{p-1} \equiv g^{p-1} \equiv 1 \pmod{p}$, 下证 $\delta_p(-g) = p-1$. 使用反证法, 假设 $k = \delta_p(-g) \leq p-2$, 则必有 $2 \nmid k$. 否则

$$g^k = (-g)^k \equiv 1 \pmod{p}, \quad \delta_p(g) = k < p-1 \text{ 矛盾.}$$

又 $k \mid p-1$, $2 \nmid k$, 得 $k \mid \frac{p-1}{2}$. 由 $p \equiv 1 \pmod{4}$, 得 $2 \mid \frac{p-1}{2}$.

从而有 $(-g)^{\frac{p-1}{2}} = g^{\frac{p-1}{2}} \equiv 1 \pmod{p}$. 与 g 为原根矛盾! 故 $k = p-1$, 即 $-g$ 为 p 的原根.